Added lemmas, need to finish rep function

examples/plane-trees/mts-different-type.dfy
@@ -57,28 +57,36 @@ function method {:opaque} R(t: TreeLB): TreeP
   NilP 
 }
 
-// Assume this when needed
-predicate R_LeftInverse()
+lemma R_LeftInverse(t: TreeP)
+  ensures R(C(t)) == t
 {
-  forall t: TreeP :: R(C(t)) == t
+  assume R(C(t)) == t;
 }
+ 
 
-// Assume this when needed 
-predicate R_Monotonicity(a: Maybe<int>, t1: TreeLB, t2: TreeLB, t1': TreeLB, t2': TreeLB)
+lemma R_Monotonicity(a: Maybe<int>, t1: TreeLB, t2: TreeLB, t1': TreeLB, t2': TreeLB)
   requires R(t1) == R(t1) && R(t2) == R(t2')
+  ensures R(NodeLB(a, t1, t2)) == R(NodeLB(a, t1', t2'))
 {
-  R(NodeLB(a, t1, t2)) == R(NodeLB(a, t1', t2'))
+  assume R(NodeLB(a, t1, t2)) == R(NodeLB(a, t1', t2'));
 }
 
 // This is \mathcal{K}
-function method Link(a: int, t1: TreeP, t2: TreeP): TreeP 
+function method Link(a: Maybe<int>, t1: TreeP, t2: TreeP): TreeP 
 {
-  R(NodeLB(Just(a), C(t1), C(t2)))
+  R(NodeLB(a, C(t1), C(t2)))
 }
 
-predicate LinkFact(a: int, t1: TreeP, t2: TreeP)
+// Don't know how to deal with this in general
+function method MaybeToInt(a: Maybe<int>): int 
 {
-  Link(a, t1, t2) == NodeP(a, Cons(t1, Cons(t2, Nil)))
+  if a.Just? then a.val else 0 
+}
+
+lemma LinkFact(a: Maybe<int>, t1: TreeP, t2: TreeP)
+  ensures Link(a, t1, t2) == NodeP(MaybeToInt(a), Cons(t1, Cons(t2, Nil)))
+{
+  assume Link(a, t1, t2) == NodeP(MaybeToInt(a), Cons(t1, Cons(t2, Nil)));
 }
 
 
@@ -126,27 +134,144 @@ function method g(t: TreeLB): (int, int)
 {
   G((0, 0), t)
 }
-
+ 
 function method G(s: (int, int), t: TreeLB): (int, int)
+  requires s.1 >= s.0
+  ensures G(s, t).1 >= G(s, t).0
   decreases t 
 {
   match t 
   {
     case NilLB => s 
-    case NodeLB(a, l, r) => G(G(OPlusG(s, a), l), r)
+    case NodeLB(a, l, r) => G(G(OPlusG(s, MaybeToInt(a)), l), r)
   }
 }
 
-function method OPlusG(s: (int, int), a: Maybe<int>): (int, int) 
+function method OPlusG(s: (int, int), a: int): (int, int) 
 {
-  var a_val := if a.Just? then a.val else 0;
-  (s.0 + a_val, Max(s.1, s.0 + a_val))
+  (s.0 + a, Max(s.1, s.0 + a))
 }
 
-/**** THE LEMMAS ****/
-
-// Assume when needed
-predicate BaseCase()
+// This is an operator introduced later. 
+// Discovering and proving that it works is outside the scope
+// of this example.
+function method OTimesG(s: (int, int), r: (int, int)): (int, int)
 {
-  
+  (s.0 + r.0, Max(s.1, s.0 + r.1))
+} 
+
+lemma OTimesOPlusLemma(s: (int, int), a: int, r: (int, int))
+  requires s.1 >= s.0 && r.1 >= r.0 
+  ensures OTimesG(OPlusG(s, a), r) == OTimesG(s, OTimesG(OPlusG((0,0), a), r))
+{
+
+}
+
+lemma OTimesGAssoc(x: (int, int), y: (int, int), z: (int, int))
+  requires x.1 >= x.0 && y.1 >= y.0 && z.1 >= z.0  
+  ensures OTimesG(OTimesG(x, y), z) == OTimesG(x, OTimesG(y, z))
+{
+
+}
+
+// Always slightly annoying to prove - the need for a 
+// predicate concerns me 
+lemma OTimesGBehaviour(s: (int, int), t: TreeLB)
+  requires s.1 >= s.0 
+  ensures G(s, t) == OTimesG(s, g(t))
+  decreases t
+{
+  match t 
+  case NilLB => {} 
+  case NodeLB(a, l, r) => {
+    var a_val := MaybeToInt(a);
+    calc == {
+      G(s, t);
+        {OTimesGBehaviour(G(OPlusG(s, a_val), l), r);}
+      OTimesG(G(OPlusG(s, a_val), l), g(r));
+      OTimesG(OTimesG(OPlusG(s, a_val), g(l)), g(r));
+        {
+          OTimesOPlusLemma(s, a_val, g(l));
+          OTimesGAssoc(s, OTimesG(OPlusG((0,0), a_val), g(l)), g(r));
+        }
+      OTimesG(s, OTimesG(OTimesG(OPlusG((0,0), a_val), g(l)), g(r)));
+    }
+  }
+}
+
+
+/**** THE LEMMAS ****/
+lemma BaseCase()
+  ensures f(R(NilLB)) == g(NilLB)
+{
+  assume f(R(NilLB)) == g(NilLB);
+}
+
+
+lemma SimplifiedProblem(a: int, r1: (int, int), r2: (int, int))
+  // requires r1.1 >= r1.0 && r2.1 >= r2.0 // in this case not required, since the problem is so simple
+  ensures OTimesG(OTimesG(OPlusG((0, 0), a), r1), r2) == OTimesF(OTimesF(OPlusF((0,0), a), r1), r2)
+{
+
+}
+
+lemma MainLemma(a: Maybe<int>, t1: TreeP, t2: TreeP)
+  ensures f(Link(a, t1, t2)) == OTimesG(OTimesG(OPlusG((0, 0), MaybeToInt(a)), f(t1)), f(t2))
+{
+  var r1, r2 := f(t1), f(t2);
+  LinkFact(a, t1, t2);
+  // Just some expanding... 
+  calc == {
+    f(Link(a, t1, t2));
+    // Nice, Dafny understands MaybeToInt 
+    F2(OPlusF((0, 0), MaybeToInt(a)), Cons(t1, Cons(t2, Nil)));
+    F2(OTimesF(OPlusF((0, 0), MaybeToInt(a)), f(t1)), Cons(t2, Nil));
+    OTimesF(OTimesF(OPlusF((0,0), MaybeToInt(a)), r1), r2);
+  }
+  SimplifiedProblem(MaybeToInt(a), r1, r2);
+}
+
+// After this lemma, just need to use R_LeftInverse...
+lemma EquivalentSchemesHelper(t': TreeLB)
+  ensures f(R(t')) == g(t')
+{
+  match t' 
+  {
+    case NilLB => {
+      BaseCase();
+    }
+    case NodeLB(a, l, r) => {
+      calc == {
+        f(R(NodeLB(a, l, r)));
+        // This justification is general
+          {
+            R_LeftInverse(R(l)); R_LeftInverse(R(r));
+            R_Monotonicity(a, l, r, C(R(l)), C(R(r)));
+          }
+        f(R(NodeLB(a, C(R(l)), C(R(r)))));
+        f(Link(a, R(l), R(r)));
+          {MainLemma(a, R(l), R(r));}
+        // Below is the g <- f term 
+        OTimesG(OTimesG(OPlusG((0, 0), MaybeToInt(a)), f(R(l))), f(R(r)));
+          {
+            EquivalentSchemesHelper(l); 
+            EquivalentSchemesHelper(r);
+          }
+        // Now we're pretty much done, just use the definitions
+        OTimesG(OTimesG(OPlusG((0, 0), MaybeToInt(a)), g(l)), g(r));
+          {OTimesGBehaviour(OTimesG(OPlusG((0, 0), MaybeToInt(a)), g(l)), r);}
+        G(OTimesG(OPlusG((0, 0), MaybeToInt(a)), g(l)), r);
+          {OTimesGBehaviour(OPlusG((0, 0), MaybeToInt(a)), l);}
+        G(G(OPlusG((0, 0), MaybeToInt(a)), l), r);
+      }
+    }
+  }
+}
+
+// Our goal
+lemma EquivalentSchemes(t: TreeP)
+  ensures f(t) == g(C(t))
+{
+  EquivalentSchemesHelper(C(t));
+  R_LeftInverse(t);
 }
